examples/scheduler/SchIAproof.v
@@ -1,4 +1,4 @@
-(* Require Import CRIS.
+Require Import CRIS.
 
 Require Import SchGInv SchHeader SchI SchA SchASpec.
 
@@ -9,7 +9,7 @@ Local Open Scope nat_scope.
 Module SchIA.
 Section SIMMODSEM.
   Import SchAS.
-  Context `{_W: @sinvGS Σ Γ α β τ, !G Γ}.
+  Context `{!sinvGS Σ Γ α β τ, !SchAS.GS Σ}.
 
   Notation iProp := (iProp Σ).
 
@@ -152,8 +152,8 @@ Section SIMMODSEM.
             ∧ <<THWF: ths_wf numths ths_tgt>>
             ∧ <<SIM: (∀ tid, sim_ths tid (alist_find tid ths_tgt) (ths_src_b tid) (ths_src_w tid) (ths_cond !! tid))>>
             ∧ <<NTHS: 0 < numths>>⌝
-          ∗ OwnM (● ths_src_b)
-          ∗ OwnM (◯ ths_src_w)
+          ∗ own sch_name (● ths_src_b)
+          ∗ own sch_name (◯ ths_src_w)
           ∗ ([∗ map] tid↦P ∈ ths_cond, P))%I.
 
   Local Notation SchAMod := (SchA.t univ StbFun StbSch).
@@ -181,23 +181,24 @@ Section SIMMODSEM.
     steps_l. forces_l. iSplitL "W PRE".
 
     { Unshelve.
-      2:{ clear H3 DT. unfold find_fsp in m. rewrite H2 in m. ss. }
+      2:{ clear H4 DT. unfold find_fsp in m. rewrite H3 in m. ss. }
       2:{ exact (q10↑). } ss.
-      unfold find_fsp in *. revert H3. revert m.
-      generalize H2. rewrite H2. i. ss.
+      unfold find_fsp in *. revert H4. revert m.
+      generalize H3. rewrite H3. i. ss.
       rewrite (@UIP _ _ _ H0 eq_refl). erewrite <-rew_swap; et. ss.
-      unfold fspec_spawnable in H3. des.
+      unfold fspec_spawnable in H4. des.
       iCombine "W PRE" as "PRE".
-      iPoseProof (H3 with "PRE") as "PRE". ss. }
+      iPoseProof (H4 with "PRE") as "PRE". ss.
+    }
 
     call "IST"; et. iModIntro. steps_l.
     rename vret into ret. rename q into vret.
 
     (* iDestruct "ASM" as "(W & % & POST)". des; subst; hss. *)
 
-    revert H3. revert m. unfold find_fsp. generalize H2. rewrite H2. i. ss.
+    revert H4. revert m. unfold find_fsp. generalize H3. rewrite H3. i. ss.
     rewrite (@UIP _ _ _ H0 eq_refl). erewrite <-rew_swap; et. ss.
-    unfold fspec_spawnable in H3. des.
+    unfold fspec_spawnable in H4. des.
     iAssert (∃ vret: Any.t, postcond x0 my_tid m vret ret)%I with "[ASM]" as "POST".
     { iExists _. et. }
 
@@ -219,46 +220,45 @@ Section SIMMODSEM.
           rewrite eq_rel_dec_correct. des_ifs. ss. des; split; et.
         - i. destruct (classic (tid = my_tid)).
           + subst. erewrite alist_replace_find_eq_None; et. 
-            rewrite -H -H0 -H4. econs 1; et. exact None.
+            rewrite -H0 -H2 -H5. econs 1; et. exact None.
           + erewrite alist_replace_find_neq_Some; et. exact None.
       }
       { (* already done case - impossible *)
         dup SIM. specialize (SIM my_tid). rewrite LU in SIM. inv SIM.
         { (* done *)
-          symmetry in H6. iCombine "TKN THW" as "X". iOwnWf "X".
-          exfalso. rewrite auth_frag_valid in H0.
-          specialize (H0 my_tid). rewrite discrete_fun_lookup_op in H0.
-          rewrite -H5 in H0. rewrite Nat.eqb_refl in H0.
-          rewrite Some_valid pair_valid in H0; des. ss.
+          symmetry in H6. iCombine "TKN THW" gives %X.
+          exfalso. rewrite auth_frag_valid in X.
+          specialize (X my_tid). rewrite discrete_fun_lookup_op in X. ss.
+          rewrite H6 in X. rewrite Nat.eqb_refl in X.
+          rewrite Some_valid pair_valid in X; des. ss.
         }
         { (* joined *) 
-          symmetry in H6. iCombine "TKN THW" as "X". iOwnWf "X".
-          exfalso. rewrite auth_frag_valid in H0.
-          specialize (H0 my_tid). rewrite discrete_fun_lookup_op in H0.
-          rewrite -H5 in H0. rewrite Nat.eqb_refl in H0.
-          rewrite Some_valid pair_valid in H0; des. ss.
+          symmetry in H6. iCombine "TKN THW" gives %X.
+          exfalso. rewrite auth_frag_valid in X.
+          specialize (X my_tid). rewrite discrete_fun_lookup_op in X. ss.
+          rewrite H6 in X. rewrite Nat.eqb_refl in X.
+          rewrite Some_valid pair_valid in X; des. ss.
         }
       }
       { (* active - only possible case *)
         dup SIM. specialize (SIM my_tid). rewrite LU in SIM. inv SIM.
-        iCombine "TKN THW" as "THW".
+        iCombine "TKN THW" gives %THW. iCombine "TKN THW" as "THW".
 
-        iOwnWf "THW".
-        rewrite auth_frag_valid in H5.
-        specialize (H5 my_tid). rewrite discrete_fun_lookup_op in H5. rewrite Nat.eqb_refl in H5.
-        rewrite -H0 in H5. rewrite// -Some_op Some_valid pair_valid in H5. des; ss.
-        apply agree_op_inv in H6.
+        rewrite auth_frag_valid in THW. ss.
+        specialize (THW my_tid). rewrite discrete_fun_lookup_op in THW. rewrite Nat.eqb_refl in THW.
+        rewrite -H2 in THW. rewrite// -Some_op Some_valid pair_valid in THW. des; ss.
+        apply agree_op_inv in THW0.
 
         remember (λ s: SAny.t, Some (to_agree (q4 s)))%I as POSTF.
         iAssert (interp_cond (Q sret))%I with "[POST]" as "POST".
-        { subst. apply (inj to_agree) in H6. specialize (H6 sret). ss. inv H6.
-          apply (inj to_agree) in H9. unfold interp_cond. rewrite H9. et. }
+        { subst. apply (inj to_agree) in THW0. specialize (THW0 sret). ss. inv THW0.
+          apply (inj to_agree) in H8. unfold interp_cond. rewrite H8. et. }
 
         assert (((((λ n : nat, if my_tid =? n then Some ((1/2)%Qp, to_agree POSTF) else ε): threadsF) ⋅ ths_src_w): threadsF) ≡ ((λ n : nat, if my_tid =? n then Some ((3/4)%Qp, to_agree (λ s: SAny.t, Some (to_agree (Q s)))) else ths_src_w n): threadsF)).
         { intros y. rewrite discrete_fun_lookup_op. des_ifs. 2:rewrite left_id //.
-          rewrite Nat.eqb_eq in Heq; subst. rewrite -H0 -Some_op -pair_op frac_op -H6 agree_idemp.
+          rewrite Nat.eqb_eq in Heq; subst. rewrite -H2 -Some_op -pair_op frac_op -THW0 agree_idemp.
           f_equiv. f_equiv. compute_done. }
-        rewrite H7.
+        rewrite H6.
 
         iExists _, _, _, (<[my_tid:=(interp_cond (Q sret))%I]> ths_cond).
         iFrame. iSplitR "POST COND".
@@ -268,7 +268,7 @@ Section SIMMODSEM.
             des; split; et.
           + i. destruct (classic (tid = my_tid)).
             * subst. erewrite alist_replace_find_eq_Some; et. rewrite !lookup_insert. 
-              rewrite Nat.eqb_refl. rewrite -H. econs 3; et.
+              rewrite Nat.eqb_refl. rewrite -H0. econs 3; et.
             * erewrite alist_replace_find_neq_Some; et. 2:exact None.
               des_ifs; [rewrite Nat.eqb_eq in Heq; subst; ss|].
               rewrite !lookup_insert_ne; et.
@@ -315,10 +315,10 @@ Section SIMMODSEM.
     iDestruct "IST" as (? ? ? ?) "(% & THB & THW & COND)". subst; hss. steps_r.
 
     (* create new token *)
-    dup THWF. apply ths_wf_nths_none in THWF. hexploit (SIM nths). i. rewrite THWF in H. inv H.
+    dup THWF. apply ths_wf_nths_none in THWF. hexploit (SIM nths). i. rewrite THWF in H0. inv H0.
 
     iCombine "THB THW" as "TH".
-    iPoseProof (OwnM_Upd with "TH") as "TH".
+    iPoseProof (own_update with "TH") as "TH".
     { apply shot_thread with (Q:=q4). split; et. apply wf_ths_src in SIM. et. }
     iApply isim_upd. iMod "TH" as "[[[[THB THW] TKNH] TKNQ1] TKNQ0]". iModIntro.
 
@@ -338,7 +338,7 @@ Section SIMMODSEM.
         des; des_ifs; split; [nia|et].
       - i. destruct (classic (tid = nths)).
         + subst. rewrite alist_add_find_eq. 
-          rewrite !discrete_fun_lookup_op Nat.eqb_refl -H1 left_id -H4.
+          rewrite !discrete_fun_lookup_op Nat.eqb_refl -H2 left_id -H5.
           econs 2; et.
         + rewrite alist_add_find_neq; et.
           rewrite discrete_fun_lookup_op.
@@ -412,37 +412,38 @@ Section SIMMODSEM.
         force_l true. steps_l. force_l. steps_l.
         iPoseProof (big_sepM_delete with "COND") as "[POST COND]"; et.
 
-        iCombine "THW TKN" as "WF". iOwnWf "WF" as WF.
-        rewrite auth_frag_valid in WF. specialize (WF q).
-        rewrite discrete_fun_lookup_op Nat.eqb_refl -H3 -Some_op Some_valid in WF.
+        iCombine "THW TKN" gives %WF. iCombine "THW TKN" as "WF".
+        rewrite auth_frag_valid in WF. specialize (WF q). ss.
+        rewrite discrete_fun_lookup_op Nat.eqb_refl -H4 -Some_op Some_valid in WF.
         rewrite -pair_op pair_valid frac_op in WF. des.
 
         apply agree_op_inv in WF0. dup WF0.
         apply (inj to_agree) in WF0.
         iAssert (interp_cond (q2 t))%I with "[POST]" as "POST".
-        { unfold interp_cond. specialize (WF0 t). ss. inv WF0. apply (inj to_agree) in H5.
-          rewrite -H5. iApply "POST". }
+        { unfold interp_cond. specialize (WF0 t). ss. inv WF0. apply (inj to_agree) in H6.
+          rewrite -H6. iApply "POST". }
         
         forces_l. iSplitL "W POST"; iFrame; et.
         assert (◯ (ths_src_w ⋅ (λ n: nat, if q =? n then Some ((1/4)%Qp, to_agree (λ s: SAny.t, Some (to_agree (q2 s)))) else ε) : threadsF) ≡ ◯ ((λ n: nat, if q =? n then Some (1%Qp, to_agree (λ s: SAny.t, Some (to_agree (Q s)))) else ths_src_w n) : threadsF)).
         { f_equiv. intros y. rewrite !discrete_fun_lookup_op.
           destruct (classic (q = y)).
           - subst. rewrite Nat.eqb_refl.
-            rewrite -WF1 -H3 -Some_op -pair_op frac_op agree_idemp. do 2 f_equiv.
+            rewrite -WF1 -H4 -Some_op -pair_op frac_op agree_idemp. do 2 f_equiv.
             compute_done.
           - des_ifs; [|rewrite right_id //]. rewrite Nat.eqb_eq in Heq. subst; ss.
-        } rewrite H0.
+        }
+        rewrite H1.
 
         step. iSplit; et. iExists _, _, _, _. iFrame. iPureIntro.
         esplits; et. i. destruct (classic (tid = q)).
-        - subst. rewrite LU -H2 Nat.eqb_refl lookup_delete. econs.
+        - subst. rewrite LU -H3 Nat.eqb_refl lookup_delete. econs.
         - des_ifs; [rewrite Nat.eqb_eq in Heq; subst; ss|].
           rewrite lookup_delete_ne; et.
       }
       { (* joined(X) *)
-        iCombine "THW TKN" as "X". iOwnWf "X" as WF. exfalso.
-        rewrite auth_frag_valid in WF. specialize (WF q).
-        rewrite discrete_fun_lookup_op -H3 Nat.eqb_refl -Some_op -pair_op frac_op in WF.
+        iCombine "THW TKN" gives %WF. exfalso.
+        rewrite auth_frag_valid in WF. specialize (WF q). ss.
+        rewrite discrete_fun_lookup_op -H4 Nat.eqb_refl -Some_op -pair_op frac_op in WF.
         rewrite Some_valid pair_valid in WF. des. ss.
       }
     }
@@ -456,11 +457,11 @@ Section SIMMODSEM.
       by_coind "CIH". iFrame.
     }
     { (* idle(X) *)
-      iCombine "THB TKN" as "X". iOwnWf "X" as WF. exfalso.
+      iCombine "THB TKN" gives %WF. exfalso.
       hexploit (SIM q). intro STHS. rewrite LU in STHS. inv STHS.
       apply auth_both_valid_discrete in WF. des.
       apply (discrete_fun_included_spec_1 _ _ q) in WF.
-      ss. rewrite Nat.eqb_refl in WF. rewrite -H0 in WF.
+      ss. rewrite Nat.eqb_refl in WF. rewrite -H1 in WF.
       eapply fragree_incl_false. et.
     }
 
@@ -491,7 +492,7 @@ Section SIMMODSEM.
 End SIMMODSEM.
 
 Section PROOF.
-  Context `{_W: @sinvGS Σ Γ α β τ, !SchAS.G Γ}.
+  Context `{_W: @sinvGS Σ Γ α β τ, !SchAS.GS Σ}.
 
   Theorem correct univ (StbFun StbSch: Sk.t -> gname -> option fspec)
     (FunInStbSch: forall sk, stb_sub (StbFun sk) (StbSch sk))
@@ -506,4 +507,4 @@ Section PROOF.
 
 End PROOF.
 
-End SchIA. *)
+End SchIA.
